use the non-dependent version by default.

src/SepTac.v
@@ -3,7 +3,71 @@ Require Import Word.
 Import List.
 Require Import Env.
 
-Require Bedrock.dep.SepExpr.
+(** Non-dependent **)
+Require Bedrock.ndep.Expr Bedrock.ndep.SepExpr.
+Module SEP := SepExpr.SepExpr BedrockHeap ST.
+
+Definition bedrock_types : list Expr.type :=
+  (** TODO: I think that we want a comparable W **)
+  {| Expr.Impl := W 
+   ; Expr.Eq := fun x y => 
+     match weq x y with
+       | left pf => Some pf 
+       | _ => None 
+     end |} :: SEP.defaultType (settings * state)%type :: nil.
+
+Lemma ApplyCancelSep : forall types funcs sfuncs (l r : SEP.sexpr (bedrock_types ++ types) (Expr.tvType O) (Expr.tvType 1)),
+  (forall cs,
+    match SEP.CancelSep cs nil l r with
+      | {| SEP.vars := vars; 
+           SEP.lhs := lhs; SEP.rhs_ex := rhs_ex; 
+           SEP.rhs := rhs; SEP.SUBST := SUBST |} =>
+           SEP.forallEach vars
+             (fun VS : Expr.env (bedrock_types ++ types) =>
+              SEP.exists_subst funcs VS
+                (ExprUnify.env_of_Subst SUBST rhs_ex 0)
+                (fun rhs_ex0 : Expr.env (bedrock_types ++ types) =>
+                 SEP.himp funcs sfuncs nil rhs_ex0 VS cs lhs rhs))
+    end) ->
+  (@SEP.sexprD _ funcs _ _ sfuncs l nil nil)
+  ===>
+  (@SEP.sexprD _ funcs _ _ sfuncs r nil nil).
+Proof.
+  unfold Himp. intros. specialize (H specs). 
+  apply SEP.ApplyCancelSep in H. unfold SEP.himp in *. assumption.
+Qed.
+
+
+Lemma Himp_to_SEP_himp : forall types funcs sfuncs 
+  (l r : @SEP.sexpr (bedrock_types ++ types) (Expr.tvType 0) (Expr.tvType 1)),
+  (forall cs, SEP.himp funcs sfuncs nil nil nil cs l r) ->
+  (@SEP.sexprD _ funcs _ _ sfuncs l nil nil)
+  ===>
+  (@SEP.sexprD _ funcs _ _ sfuncs r nil nil).
+Proof.
+  unfold Himp, SEP.himp. intuition.
+Qed.
+
+Ltac reflect_goal isConst Ts :=
+  match goal with 
+    | [ |- Himp ?L ?R ] =>
+      let pcT := constr:(W) in
+      let stateT := constr:(prod settings state) in
+      let Ts := eval unfold bedrock_types in bedrock_types in
+      let goals := constr:(L :: R :: nil) in
+      let goals := eval unfold starB exB hvarB in goals in
+      let v := SEP.reflect_all pcT stateT ltac:(isConst) Ts goals in
+      match v with
+        | (?types, ?pcT, ?stT, ?funcs, ?sfuncs, ?L :: ?R :: nil) => 
+          apply (@Himp_to_SEP_himp _ funcs sfuncs L R)
+      end
+  end.
+
+
+(*
+(** Dependent **)
+
+Require Bedrock.dep.Expr Bedrock.dep.SepExpr.
 Module SEP := SepExpr.SepExpr BedrockHeap ST.
 
 Definition bedrock_types : list Expr.type :=
@@ -57,5 +121,4 @@ Ltac reflect_goal isConst Ts :=
           eapply (@Himp_to_SEP_himp _ _ _ L R)
       end
   end.
-
-
+*)
